Fix false predicate Wellformed

isa.dfy
@@ -41,7 +41,7 @@ datatype ProcessingElement =
 
     // Get the input channel indices a PE is currently waiting on
     function method WaitingInputs(): seq<ChannelIndex>
-        ensures multiset(WaitingInputs()) <= multiset(Inputs())
+        ensures forall i :: i in WaitingInputs() ==> i in Inputs()
     {
         match this {
             case AddOperator(a, b, _) => [a, b]
@@ -65,24 +65,26 @@ datatype ProcessingElement =
     }
 }
 
-datatype Channel = Channel(buffer: seq<Value>)
-{
-    function method Length(): int
-    {
-        |buffer|
-    }
+type Channel = seq<Value>
 
-    function method Send(value: Value): (newChannel: Channel)
-    {
-        Channel(buffer + [value])
-    }
+// datatype Channel = Channel(buffer: seq<Value>)
+// {
+//     function method Length(): int
+//     {
+//         |buffer|
+//     }
 
-    function method Receive(): (Value, Channel)
-        requires |buffer| > 0
-    {
-        (buffer[0], Channel(buffer[1..]))
-    }
-}
+//     function method Send(value: Value): (newChannel: Channel)
+//     {
+//         Channel(buffer + [value])
+//     }
+
+//     function method Receive(): (Value, Channel)
+//         requires |buffer| > 0
+//     {
+//         (buffer[0], Channel(buffer[1..]))
+//     }
+// }
 
 datatype DataflowProgramState = DataflowProgramState(channels: seq<Channel>, processingElements: seq<ProcessingElement>)
 {
@@ -95,28 +97,28 @@ datatype DataflowProgramState = DataflowProgramState(channels: seq<Channel>, pro
         // Each node has distinct input channels
 
         var validChannelIndices :=
-            forall pe :: pe in processingElements[..] ==>
+            forall pe :: pe in processingElements ==>
             forall idx :: idx in pe.Inputs() || idx in pe.Outputs() ==>
             0 <= idx < |channels|;
 
         var noIOOverlap := 
-            forall pe1 :: pe1 in processingElements[..] ==>
-            forall pe2 :: pe2 in processingElements[..] && pe1 != pe2 ==>
-                multiset(pe1.Inputs()) * multiset(pe2.Inputs()) == multiset{} &&
-                multiset(pe1.Outputs()) * multiset(pe2.Outputs()) == multiset{};
+            forall pe1 :: pe1 in processingElements ==>
+            forall pe2 :: pe2 in processingElements && pe1 != pe2 ==>
+                (forall i :: i in pe1.Inputs() ==> i !in pe2.Inputs()) &&
+                (forall i :: i in pe1.Outputs() ==> i !in pe2.Outputs());
 
         var distinctPEs :=
             forall i, j :: 0 <= i < j < |processingElements| ==>
             processingElements[i] != processingElements[j];
 
         var distinctInputChannels :=
-            forall pe :: pe in processingElements[..] ==>
+            forall pe :: pe in processingElements ==>
             forall i, j :: 0 <= i < j < |pe.Inputs()| ==>
             pe.Inputs()[i] != pe.Inputs()[j];
 
         var distinctOutputChannels :=
-            forall pe :: pe in processingElements[..] ==>
-            forall i, j :: 0 <= i < |pe.Outputs()| && 0 <= j < |pe.Outputs()| ==>
+            forall pe :: pe in processingElements ==>
+            forall i, j :: 0 <= i < j < |pe.Outputs()| ==>
             pe.Outputs()[i] != pe.Outputs()[j];
 
         validChannelIndices && noIOOverlap && distinctPEs && distinctInputChannels && distinctOutputChannels
@@ -129,7 +131,7 @@ datatype DataflowProgramState = DataflowProgramState(channels: seq<Channel>, pro
     {
         forall ChannelIndex :: ChannelIndex in processingElements[idx].WaitingInputs() ==>
             ChannelIndex in processingElements[idx].Inputs() && // TODO: this is not necessary
-            channels[ChannelIndex].Length() != 0
+            |channels[ChannelIndex]| != 0
     }
 
     function Multicast(value: Value, outputs: seq<ChannelIndex>): DataflowProgramState
@@ -142,7 +144,7 @@ datatype DataflowProgramState = DataflowProgramState(channels: seq<Channel>, pro
                 result.processingElements == processingElements &&
                 forall idx :: 0 <= idx < |channels| ==>
                     (idx !in outputs ==> result.channels[idx] == channels[idx]) &&
-                    (idx in outputs ==> result.channels[idx] == channels[idx].Send(value))
+                    (idx in outputs ==> result.channels[idx] == channels[idx] + [value])
 
         decreases outputs
     {
@@ -151,7 +153,7 @@ datatype DataflowProgramState = DataflowProgramState(channels: seq<Channel>, pro
         else
             var idx := outputs[0];
             assert idx in outputs;
-            var newChannels := channels[idx := channels[idx].Send(value)];
+            var newChannels := channels[idx := channels[idx] + [value]];
             var newState := DataflowProgramState(newChannels, processingElements);
             assert forall idx :: idx in outputs[1..] ==> idx in outputs;
             newState.Multicast(value, outputs[1..])
@@ -162,6 +164,7 @@ datatype DataflowProgramState = DataflowProgramState(channels: seq<Channel>, pro
         requires 0 <= idx < |processingElements|
         requires Wellformed()
         requires IsFireable(idx)
+
         ensures Wellformed()
         ensures |result.channels| == |channels|
         ensures |result.processingElements| == |processingElements|
@@ -169,8 +172,11 @@ datatype DataflowProgramState = DataflowProgramState(channels: seq<Channel>, pro
         ensures result.processingElements[idx].Inputs() == processingElements[idx].Inputs()
         ensures result.processingElements[idx].Outputs() == processingElements[idx].Outputs()
 
+        ensures forall i :: 0 <= i < |result.processingElements| && i != idx
+                            ==> result.processingElements[i] == processingElements[i]
+
         ensures forall i :: 0 <= i < |result.channels| &&
-                            i !in processingElements[idx].Inputs() &&
+                            i !in processingElements[idx].WaitingInputs() &&
                             i !in processingElements[idx].Outputs() ==> result.channels[i] == channels[i]
     {
         var pe := processingElements[idx];
@@ -181,9 +187,9 @@ datatype DataflowProgramState = DataflowProgramState(channels: seq<Channel>, pro
                 // assert a == pe.Inputs()[0] && b == pe.Inputs()[1];
                 // assert a != b;
 
-                var (valA, newChannelA) := channels[a].Receive();
-                var (valB, newChannelB) := channels[b].Receive();
-                var newChannels := channels[a := newChannelA][b := newChannelB];
+                var valA := channels[a][0];
+                var valB := channels[b][0];
+                var newChannels := channels[a := channels[a][1..]][b := channels[b][1..]];
                 var newState := DataflowProgramState(newChannels, processingElements);
 
                 newState.Multicast(valA + valB, outputs)
@@ -192,9 +198,9 @@ datatype DataflowProgramState = DataflowProgramState(channels: seq<Channel>, pro
                 assert d in pe.Inputs() && a in pe.Inputs();
                 assert outputs <= pe.Outputs();
 
-                var (valD, newChannelD) := channels[d].Receive();
-                var (valA, newChannelA) := channels[a].Receive();
-                var newChannels := channels[d := newChannelD][a := newChannelA];
+                var valD := channels[d][0];
+                var valA := channels[a][0];
+                var newChannels := channels[d := channels[d][1..]][a := channels[a][1..]];
                 var newState := DataflowProgramState(newChannels, processingElements);
 
                 if valD == 1 then
@@ -206,9 +212,9 @@ datatype DataflowProgramState = DataflowProgramState(channels: seq<Channel>, pro
                 assert d in pe.Inputs() && a in pe.Inputs();
                 assert outputs <= pe.Outputs();
 
-                var (valD, newChannelD) := channels[d].Receive();
-                var (valA, newChannelA) := channels[a].Receive();
-                var newChannels := channels[d := newChannelD][a := newChannelA];
+                var valD := channels[d][0];
+                var valA := channels[a][0];
+                var newChannels := channels[d := channels[d][1..]][a := channels[a][1..]];
                 var newState := DataflowProgramState(newChannels, processingElements);
 
                 if valD == 0 then
@@ -220,10 +226,10 @@ datatype DataflowProgramState = DataflowProgramState(channels: seq<Channel>, pro
                 assert d in pe.Inputs() && a in pe.Inputs() && b in pe.Inputs();
                 assert outputs <= pe.Outputs();
 
-                var (valD, newChannelD) := channels[d].Receive();
-                var (valA, newChannelA) := channels[a].Receive();
-                var (valB, newChannelB) := channels[b].Receive();
-                var newChannels := channels[d := newChannelD][a := newChannelA][b := newChannelB];
+                var valD := channels[d][0];
+                var valA := channels[a][0];
+                var valB := channels[b][0];
+                var newChannels := channels[d := channels[d][1..]][a := channels[a][1..]][b := channels[b][1..]];
                 var newState := DataflowProgramState(newChannels, processingElements);
 
                 if valD == 1 then
@@ -236,19 +242,21 @@ datatype DataflowProgramState = DataflowProgramState(channels: seq<Channel>, pro
                     case CarryI =>
                         assert a in pe.Inputs();
 
-                        var (valA, newChannelA) := channels[a].Receive();
-                        var newChannels := channels[a := newChannelA];
+                        var valA := channels[a][0];
+                        var newChannels := channels[a := channels[a][1..]];
                         var newPEs := processingElements[idx := CarryOperator(CarryB1, d, a, b, outputs)];
                         var newState := DataflowProgramState(newChannels, newPEs);
 
                         assert forall i :: 0 <= i < |newPEs| ==> newPEs[i].Inputs() == processingElements[i].Inputs();
+                        assert processingElements[idx].Outputs() == outputs;
+
                         newState.Multicast(valA, outputs)
 
                     case CarryB1 =>
                         assert d in pe.Inputs();
 
-                        var (valD, newChannelD) := channels[d].Receive();
-                        var newChannels := channels[d := newChannelD];
+                        var valD := channels[d][0];
+                        var newChannels := channels[d := channels[d][1..]];
 
                         var updatedPE := if valD == 0 then CarryOperator(CarryI, d, a, b, outputs)
                                                       else CarryOperator(CarryB2, d, a, b, outputs);
@@ -259,12 +267,14 @@ datatype DataflowProgramState = DataflowProgramState(channels: seq<Channel>, pro
                     case CarryB2 =>
                         assert b in pe.Inputs();
 
-                        var (valB, newChannelB) := channels[b].Receive();
-                        var newChannels := channels[b := newChannelB];
+                        var valB := channels[b][0];
+                        var newChannels := channels[b := channels[b][1..]];
                         var newPEs := processingElements[idx := CarryOperator(CarryB1, d, a, b, outputs)];
                         var newState := DataflowProgramState(newChannels, newPEs);
 
                         assert forall i :: 0 <= i < |newPEs| ==> newPEs[i].Inputs() == processingElements[i].Inputs();
+                        assert processingElements[idx].Outputs() == outputs;
+
                         newState.Multicast(valB, outputs)
                 }
 
@@ -272,9 +282,9 @@ datatype DataflowProgramState = DataflowProgramState(channels: seq<Channel>, pro
                 assert a in pe.Inputs() && b in pe.Inputs();
                 assert outputs <= pe.Outputs();
                 
-                var (valA, newChannelA) := channels[a].Receive();
-                var (valB, newChannelB) := channels[b].Receive();
-                var newChannels := channels[a := newChannelA][b := newChannelB];
+                var valA := channels[a][0];
+                var valB := channels[b][0];
+                var newChannels := channels[a := channels[a][1..]][b := channels[b][1..]];
                 var newState := DataflowProgramState(newChannels, processingElements);
 
                 newState.Multicast(valB, outputs)
@@ -284,8 +294,8 @@ datatype DataflowProgramState = DataflowProgramState(channels: seq<Channel>, pro
                     case MergeI =>
                         assert d in pe.Inputs();
 
-                        var (valD, newChannelD) := channels[d].Receive();
-                        var newChannels := channels[d := newChannelD];
+                        var valD := channels[d][0];
+                        var newChannels := channels[d := channels[d][1..]];
 
                         var updatedPE := if valD == 0 then MergeOperator(MergeA, d, a, b, outputs)
                                                       else MergeOperator(MergeB, d, a, b, outputs);
@@ -296,26 +306,28 @@ datatype DataflowProgramState = DataflowProgramState(channels: seq<Channel>, pro
                     case MergeA =>
                         assert a in pe.Inputs();
 
-                        var (valA, newChannelA) := channels[a].Receive();
-                        var newChannels := channels[a := newChannelA];
+                        var valA := channels[a][0];
+                        var newChannels := channels[a := channels[a][1..]];
                         var newPEs := processingElements[idx := MergeOperator(MergeI, d, a, b, outputs)];
                         var newState := DataflowProgramState(newChannels, newPEs);
 
                         assert forall i :: 0 <= i < |newPEs| ==> newPEs[i].Inputs() == processingElements[i].Inputs();
+                        assert processingElements[idx].Outputs() == outputs;
+
                         newState.Multicast(valA, outputs)
 
                     case MergeB =>
                         assert b in pe.Inputs();
+                        assert outputs <= pe.Outputs();
 
-                        var (valB, newChannelB) := channels[b].Receive();
-                        var newChannels := channels[b := newChannelB];
+                        var valB := channels[b][0];
+                        var newChannels := channels[b := channels[b][1..]];
                         var newPEs := processingElements[idx := MergeOperator(MergeI, d, a, b, outputs)];
                         var newState := DataflowProgramState(newChannels, newPEs);
 
                         assert forall i :: 0 <= i < |newPEs| ==> newPEs[i].Inputs() == processingElements[i].Inputs();
                         newState.Multicast(valB, outputs)
                 }
-
     }
 
     predicate AreBothFireable(idx1: PEIndex, idx2: PEIndex)
@@ -328,18 +340,146 @@ datatype DataflowProgramState = DataflowProgramState(channels: seq<Channel>, pro
 
     lemma CommutableFiring(idx1: PEIndex, idx2: PEIndex)
         requires Wellformed()
-        requires AreBothFireable(idx1, idx2)
         requires idx1 != idx2
+        requires 0 <= idx1 < |processingElements|
+        requires 0 <= idx2 < |processingElements|
+        requires IsFireable(idx1)
+        requires IsFireable(idx2)
         ensures FirePE(idx1).IsFireable(idx2)
+    {}
+
+    // Output values do not depend on the channels other than WaitingInputs()
+    lemma FirePEDependency(state1: DataflowProgramState, state2: DataflowProgramState, idx: PEIndex)
+        requires state1.Wellformed() && state2.Wellformed()
+        requires |state1.channels| == |state2.channels|
+        requires 0 <= idx < |state1.processingElements| == |state2.processingElements|
+        requires state1.processingElements[idx] == state2.processingElements[idx]
+        requires state1.IsFireable(idx) && state2.IsFireable(idx)
+
+        // Same input channels
+        requires forall i :: i in state1.processingElements[idx].WaitingInputs() ==>
+                             state1.channels[i] == state2.channels[i]
+
+        // Same output channels
+        requires forall i :: i in state1.processingElements[idx].Outputs() ==>
+                             state1.channels[i] == state2.channels[i]
+
+        // Would result in the same output input channels
+        ensures var result1 := state1.FirePE(idx);
+                var result2 := state2.FirePE(idx);
+                forall i :: i in state1.processingElements[idx].WaitingInputs() ||
+                            i in state1.processingElements[idx].Outputs() ==>
+                            result1.channels[i] == result2.channels[i]
+
+        // And the same final state for the fired PE
+        ensures state1.FirePE(idx).processingElements[idx] == state2.FirePE(idx).processingElements[idx]
+    {}
+
+    // Output values do not depend on the channels other than WaitingInputs()
+    lemma FirePEDependency2(state1: DataflowProgramState, state2: DataflowProgramState, idx: PEIndex)
+        requires state1.Wellformed() && state2.Wellformed()
+        requires |state1.channels| == |state2.channels|
+        requires 0 <= idx < |state1.processingElements| == |state2.processingElements|
+        requires state1.processingElements[idx] == state2.processingElements[idx]
+        requires state1.IsFireable(idx) && state2.IsFireable(idx)
+
+        // Same input values
+        requires forall i :: i in state1.processingElements[idx].WaitingInputs() ==>
+                             state1.channels[i][0] == state2.channels[i][0]
+
+        // Same output channels
+        // requires forall i :: i in state1.processingElements[idx].Outputs() ==>
+        //                      state1.channels[i] == state2.channels[i]
+
+        // Would result in the same "output values"
+        ensures var pe := state1.processingElements[idx];
+                var result1 := state1.FirePE(idx);
+                var result2 := state2.FirePE(idx);
+                forall i :: i in pe.Outputs() ==>
+                    // If the output channel is not an input channel
+                    (i !in pe.WaitingInputs() ==>
+                        // Either unchanged
+                        (result1.channels[i] == state1.channels[i] && result2.channels[i] == state2.channels[i]) ||
+                        // Or appended with the same value
+                        (result1.channels[i][|result1.channels[i]| - 1] == result2.channels[i][|result2.channels[i]| - 1] &&
+                         result1.channels[i][..|result1.channels[i]| - 1] == state1.channels[i] &&
+                         result2.channels[i][..|result2.channels[i]| - 1] == state2.channels[i])
+                    ) ||
+                    // Otherwise the output channel is an input channel
+                    (i in pe.WaitingInputs() ==>
+                        // Either has one value popped
+                        (result1.channels[i] == state1.channels[i][1..] && result2.channels[i] == state2.channels[i][1..]) ||
+                        // Or has one value popped and appended with the a value identical in result1 and result2
+                        (result1.channels[i][|result1.channels[i]| - 1] == result2.channels[i][|result2.channels[i]| - 1] &&
+                         result1.channels[i][..|result1.channels[i]| - 1] == state1.channels[i][1..] &&
+                         result2.channels[i][..|result2.channels[i]| - 1] == state2.channels[i][1..])
+                    )
+
+        // And the same final state for the fired PE
+        ensures state1.FirePE(idx).processingElements[idx] == state2.FirePE(idx).processingElements[idx]
     {}
 
     // This might need longer timeouts
     lemma FirePEConfluence(idx1: PEIndex, idx2: PEIndex)
         requires Wellformed()
-        requires AreBothFireable(idx1, idx2)
         requires idx1 != idx2
-        ensures FirePE(idx1).FirePE(idx2) == FirePE(idx2).FirePE(idx1)
+        requires 0 <= idx1 < |processingElements|
+        requires 0 <= idx2 < |processingElements|
+        requires IsFireable(idx1)
+        requires IsFireable(idx2)
+        // ensures FirePE(idx1).FirePE(idx2) == FirePE(idx2).FirePE(idx1)
     {
         CommutableFiring(idx1, idx2);
+        CommutableFiring(idx2, idx1);
+
+        var fired1 := FirePE(idx1);
+        var fired2 := FirePE(idx2);
+        var fired12 := fired1.FirePE(idx2);
+        var fired21 := fired2.FirePE(idx1);
+
+        var inputs1 := processingElements[idx1].WaitingInputs();
+        var inputs2 := processingElements[idx2].WaitingInputs();
+        var outputs1 := processingElements[idx1].Outputs();
+        var outputs2 := processingElements[idx2].Outputs();
+
+        assert forall i :: i in inputs1 ==> i !in inputs2;
+        assert forall i :: i in outputs1 ==> i !in outputs2;
+
+        assert forall i :: 0 <= i < |channels| &&
+                           i !in inputs1 &&
+                           i !in inputs2 &&
+                           i !in outputs1 &&
+                           i !in outputs2 ==>
+               fired12.channels[i] == fired21.channels[i] == channels[i];
+
+        assume forall i :: i in inputs1 ==> i !in outputs2;
+        assume forall i :: i in inputs2 ==> i !in outputs1;
+
+        // assert forall i :: i in inputs1 ==> fired12.channels[i] == fired1.channels[i];
+        // assert forall i :: i in outputs1 ==> fired12.channels[i] == fired1.channels[i];
+        // assert forall i :: i in inputs2 ==> fired21.channels[i] == fired2.channels[i];
+        // assert forall i :: i in outputs2 ==> fired21.channels[i] == fired2.channels[i];
+
+        // assert forall i :: i in inputs1 ==> fired2.channels[i] == channels[i];
+        // assert forall i :: i in outputs1 ==> fired2.channels[i] == channels[i];
+
+        FirePEDependency2(fired2, this, idx1);
+        FirePEDependency2(fired1, this, idx2);
+
+        assert forall i :: i in inputs1 ==> fired21.channels[i] == fired1.channels[i];
+        // assert forall i :: i in outputs1 ==> fired21.channels[i] == fired1.channels[i];
+
+        // assert forall i :: 0 <= i < |channels| && i in outputs2 ==>
+        //        fired21.channels[i] == fired2.channels[i];
+
+        // match (processingElements[idx1], processingElements[idx2]) {
+        //     case (AddOperator(_, _, _), AddOperator(_, _, _)) => {
+                
+        //     }
+        //     // case (AddOperator(_, _, _), CarryOperator(_, _, _, _, _)) => {}
+        //     // case (CarryOperator(_, _, _, _, _), AddOperator(_, _, _)) => {}
+        //     // case (CarryOperator(_, _, _, _, _), CarryOperator(_, _, _, _, _)) => {}
+        //     case _ => {}
+        // }
     }
 }
